theories/Unshadow.v
@@ -2,6 +2,7 @@ From LinearCore Require
   NewNames
   Rename
   Term
+  WellFormed
   .
 From LinearCore Require Import
   DollarSign
@@ -10,67 +11,33 @@ From LinearCore Require Import
 
 
 
-Definition get_or_add m reserved k :=
-  match Map.find m k with
-  | Some v => (m, reserved, v)
-  | None =>
-      let v := NewNames.new_name reserved k in
-      (Map.overriding_add k v m, Map.set_add v reserved, v)
-  end.
-Arguments get_or_add m reserved k/.
-
-Definition get_or_add_det {m1 r1 k1 m1' r1' v1} (E1 : get_or_add m1 r1 k1 = (m1', r1', v1))
-  {m2} (Em : Map.Eq m1 m2)
-  {r2} (Er : Map.Eq r1 r2)
-  {k2} (Ek : k1 = k2)
-  {m2' r2' v2} (E2 : get_or_add m2 r2 k2 = (m2', r2', v2))
-  : Map.Eq m1' m2' /\ Map.Eq r1' r2' /\ v1 = v2.
-Proof.
-  subst. rename k2 into k. unfold get_or_add in *. destruct (Map.find_spec m1 k).
-  - apply Em in Y. apply Map.find_iff in Y. rewrite Y in E2. clear Y. invert E1. invert E2.
-    split. { exact Em. } split. { exact Er. } reflexivity.
-  - destruct (Map.find_spec m2 k). { apply Em in Y. apply N in Y as []. }
-    invert E1. invert E2. split. { split; intro F; apply Map.find_overriding_add;
-      (apply Map.find_overriding_add in F as [[-> ->] | [Nf F]]; [left | right];
-      [split; [reflexivity |]; apply NewNames.new_name_det |
-        split; [exact Nf |]; apply Em; exact F ]); [| apply Map.eq_sym]; exact Er. }
-    split. 2: { apply NewNames.new_name_det. exact Er. }
-    split; intro F; apply Map.find_overriding_add; (
-      apply Map.find_overriding_add in F as [[-> ->] | [Nf F]]; [left | right];
-      [split; [| reflexivity]; apply NewNames.new_name_det |
-        split; [| apply Er; exact F]; intros ->; apply Nf; apply NewNames.new_name_det]);
-    try exact Er; apply Map.eq_sym; exact Er.
-Qed.
-
-
-
-Definition map3 {A B X Y} (f : X -> Y) (tuple : A * B * X) : A * B * Y :=
-  match tuple with (a, b, x) => (a, b, f x) end.
-
 (* NOTE: Even though it's a very unusual case, this has to return an option
  * because patterns (in `Cas`) can be ill-formed if they duplicate a binder. *)
 Fixpoint unshadow_acc (acc : Map.to String.string) (reserved : Map.set) t :=
   match t with
-  | Term.Ctr ctor => Some (acc, reserved, Term.Ctr ctor)
-  | Term.Mov k => Some $ map3 Term.Mov $ get_or_add acc reserved k
-  | Term.Ref k => Some $ map3 Term.Ref $ get_or_add acc reserved k
+  | Term.Ctr ctor => Some (reserved, Term.Ctr ctor)
+  | Term.Mov k =>
+      (* Have to supply a plan for any free variables (or they have to have been bound & added to the plan): *)
+      match Map.find acc k with None => None | Some v => Some (reserved, Term.Mov v) end
+  | Term.Ref k =>
+      match Map.find acc k with None => None | Some v => Some (reserved, Term.Ref v) end
   | Term.App f a =>
-      match unshadow_acc acc reserved f with None => None | Some (acc, reserved, f') =>
-        match unshadow_acc acc reserved a with None => None | Some (acc, reserved, a') =>
-          Some (acc, reserved, Term.App f' a')
+      match unshadow_acc acc reserved f with None => None | Some (reserved, f') =>
+        match unshadow_acc acc reserved a with None => None | Some (reserved, a') =>
+          Some (reserved, Term.App f' a')
         end
       end
   | Term.For variable type body =>
-      match unshadow_acc acc reserved type with None => None | Some (acc, reserved, type') =>
+      match unshadow_acc acc reserved type with None => None | Some (reserved, type') =>
         let variable' := NewNames.new_name reserved variable in
         let acc := Map.overwrite variable variable' acc in
         let reserved := Map.set_add variable' reserved in
-        match unshadow_acc acc reserved body with None => None | Some (acc, reserved, body') =>
-          Some (acc, reserved, Term.For variable' type' body')
+        match unshadow_acc acc reserved body with None => None | Some (reserved, body') =>
+          Some (reserved, Term.For variable' type' body')
         end
       end
   | Term.Cas pattern body_if_match other_cases =>
-      match unshadow_acc acc reserved other_cases with None => None | Some (acc, reserved, other_cases') =>
+      match unshadow_acc acc reserved other_cases with None => None | Some (reserved, other_cases') =>
         let bindings := BoundIn.pattern pattern in
         let rebindings := NewNames.generate reserved bindings in
         match Rename.pattern rebindings pattern with
@@ -78,69 +45,24 @@ Fixpoint unshadow_acc (acc : Map.to String.string) (reserved : Map.set) t :=
         | Some pattern' =>
             let acc := Map.bulk_overwrite rebindings acc in
             let reserved := Map.set_union (Map.range rebindings) reserved in
-            match unshadow_acc acc reserved body_if_match with None => None | Some (acc, reserved, body_if_match') =>
-              Some (acc, reserved, Term.Cas pattern' body_if_match' other_cases')
+            match unshadow_acc acc reserved body_if_match with None => None | Some (reserved, body_if_match') =>
+              Some (reserved, Term.Cas pattern' body_if_match' other_cases')
             end
         end
       end
   end.
 
-Definition unshadow reserved t :=
-  match unshadow_acc (Map.to_self reserved) reserved t with
-  | None => None
-  | Some (_, used_in_unshadowed (* cool huh *), unshadowed) => Some unshadowed
-  end.
+Definition unshadow reserved t := option_map snd $ unshadow_acc (Map.to_self reserved) reserved t.
 Arguments unshadow reserved t/.
 
 
 
-(* Rewriting without opening a can of worms: *)
-Lemma unshadow_acc_for acc reserved variable type body
-  : unshadow_acc acc reserved (Term.For variable type body) =
-    match unshadow_acc acc reserved type with
-    | None => None
-    | Some (acc', reserved', type') =>
-        match
-          unshadow_acc
-            (Map.overwrite variable (NewNames.new_name reserved' variable) acc')
-            (Map.set_add (NewNames.new_name reserved' variable) reserved') body
-        with
-        | None => None
-        | Some (acc'', reserved'', body') =>
-            Some
-              (acc'', reserved'',
-              Term.For (NewNames.new_name reserved' variable) type' body')
-        end
-    end.
-Proof. reflexivity. Qed.
-
-Lemma unshadow_acc_cas acc reserved pattern body_if_match other_cases
-  : unshadow_acc acc reserved (Term.Cas pattern body_if_match other_cases) =
-    match unshadow_acc acc reserved other_cases with None => None | Some (acc, reserved, other_cases') =>
-      match Rename.pattern (NewNames.generate reserved $ BoundIn.pattern pattern) pattern with
-      | None => None
-      | Some pattern' =>
-          match
-            unshadow_acc
-              (Map.bulk_overwrite (NewNames.generate reserved $ BoundIn.pattern pattern) acc)
-              (Map.set_union (Map.range (NewNames.generate reserved $ BoundIn.pattern pattern)) reserved)
-              body_if_match
-          with
-          | None => None
-          | Some (acc'', reserved'', body_if_match') =>
-              Some (acc'', reserved'', Term.Cas pattern' body_if_match' other_cases')
-          end
-      end
-    end.
-Proof. cbn. reflexivity. Qed.
-
-Variant Equiv : option (Map.to String.string * Map.set * Term.term) -> _ -> Prop :=
+Variant Equiv : option (Map.set * Term.term) -> _ -> Prop :=
   | ENone
       : Equiv None None
   | ESome
-      {acc1 acc2} (Eacc : Map.Eq acc1 acc2)
       {reserved1 reserved2} (Ereserved : Map.Eq reserved1 reserved2) output
-      : Equiv (Some (acc1, reserved1, output)) (Some (acc2, reserved2, output))
+      : Equiv (Some (reserved1, output)) (Some (reserved2, output))
   .
 
 Lemma det_acc
@@ -150,55 +72,68 @@ Lemma det_acc
   : Equiv (unshadow_acc a1 r1 t1) (unshadow_acc a2 r2 t2).
 Proof.
   subst. rename t2 into t. generalize dependent r2. generalize dependent r1.
-  generalize dependent a2. generalize dependent a1. induction t; intros.
-  - cbn. constructor; assumption.
-  - unfold unshadow_acc.
-    destruct (get_or_add a1 r1 name) as [[a1'' r1''] t1] eqn:E1.
-    destruct (get_or_add a2 r2 name) as [[a2'' r2''] t2] eqn:E2.
-    destruct (get_or_add_det E1 Ea Er eq_refl E2) as [Ea'' [Er'' ->]].
-    cbn. constructor; assumption.
-  - unfold unshadow_acc.
-    destruct (get_or_add a1 r1 name) as [[a1'' r1''] t1] eqn:E1.
-    destruct (get_or_add a2 r2 name) as [[a2'' r2''] t2] eqn:E2.
-    destruct (get_or_add_det E1 Ea Er eq_refl E2) as [Ea'' [Er'' ->]].
-    cbn. constructor; assumption.
-  - cbn. destruct (IHt1 _ _ Ea _ _ Er). { constructor. }
-    destruct (IHt2 _ _ Eacc _ _ Ereserved); constructor; eassumption.
-  - repeat rewrite unshadow_acc_for. destruct (IHt1 _ _ Ea _ _ Er). { constructor. }
-    assert (Ea' : Map.Eq
-      (Map.overwrite variable (NewNames.new_name reserved1 variable) acc1)
-      (Map.overwrite variable (NewNames.new_name reserved2 variable) acc2)). {
-      split; intro F; apply Map.find_overriding_add;
-      (apply Map.find_overriding_add in F as [[-> ->] | [N F]]; [left | right];
-      [split; [reflexivity |]; apply NewNames.new_name_det |
-        split; [exact N |]; apply Eacc; exact F]); [| apply Map.eq_sym]; exact Ereserved. }
-    assert (Er' : Map.Eq
-      (Map.set_add (NewNames.new_name reserved1 variable) reserved1)
-      (Map.set_add (NewNames.new_name reserved2 variable) reserved2)). {
-      split; intro F; apply Map.find_overriding_add;
-      (apply Map.find_overriding_add in F as [[-> ->] | [N F]]; [left | right];
+  generalize dependent a2. generalize dependent a1. { induction t; intros; cbn in *.
+  - constructor; assumption.
+  - unfold unshadow_acc. destruct (Map.find_spec a1 name).
+    + apply Ea in Y. apply Map.find_iff in Y. rewrite Y. constructor. exact Er.
+    + destruct (Map.find_spec a2 name). { apply Ea in Y. apply N in Y as []. } constructor.
+  - unfold unshadow_acc. destruct (Map.find_spec a1 name).
+    + apply Ea in Y. apply Map.find_iff in Y. rewrite Y. constructor. exact Er.
+    + destruct (Map.find_spec a2 name). { apply Ea in Y. apply N in Y as []. } constructor.
+  - destruct (IHt1 _ _ Ea _ _ Er). { constructor. }
+    destruct (IHt2 _ _ Ea _ _ Ereserved); constructor; eassumption.
+  - destruct (IHt1 _ _ Ea _ _ Er). { constructor. } eassert (Ea' : _); [| eassert (Er' : _); [| destruct (IHt2
+      (Map.overriding_add variable (NewNames.new_name reserved1 variable) a1)
+      (Map.overriding_add variable (NewNames.new_name reserved2 variable) a2) Ea'
+      (Map.overriding_add (NewNames.new_name reserved1 variable) tt reserved1)
+      (Map.overriding_add (NewNames.new_name reserved2 variable) tt reserved2) Er')]]. 3: { constructor. }
+    + split; intro F; apply Map.find_overriding_add; (apply Map.find_overriding_add in F as [[-> ->] | [N F]]; [left | right];
+      [split; [reflexivity | apply NewNames.new_name_det] | split; [exact N |]; apply Ea; exact F]); [| apply Map.eq_sym]; exact Ereserved.
+    + split; intro F; apply Map.find_overriding_add; (apply Map.find_overriding_add in F as [[-> ->] | [N F]]; [left | right];
       [split; [| reflexivity]; apply NewNames.new_name_det | split; [| apply Ereserved; exact F];
-        intros ->; apply N; apply NewNames.new_name_det]);
-      try exact Ereserved; apply Map.eq_sym; exact Ereserved. }
-    destruct (IHt2 _ _ Ea' _ _ Er'). { constructor. }
-    erewrite NewNames.new_name_det; [constructor |]. { exact Eacc0. } { exact Ereserved0. } exact Ereserved.
-  - repeat rewrite unshadow_acc_cas. destruct (IHt2 _ _ Ea _ _ Er). { constructor. }
-    erewrite NewNames.generate_det. 2: { exact Ereserved. } 2: { apply Map.eq_refl. }
-    eassert (O2O : Map.OneToOne $ NewNames.generate reserved2 (BoundIn.pattern pattern)). {
-      apply NewNames.one_to_one_generate. } destruct (Rename.pattern_spec O2O pattern). 2: { constructor. }
-    eassert (Ea' : Map.Eq
-      (Map.bulk_overwrite (NewNames.generate reserved2 (BoundIn.pattern pattern)) acc1)
-      (Map.bulk_overwrite (NewNames.generate reserved2 (BoundIn.pattern pattern)) acc2)). {
-      split; intro F; apply Map.bulk_overwrite_bulk_overwrite; (
-      apply Map.bulk_overwrite_bulk_overwrite in F as [F | [N F]]; [left; exact F | right]);
-      (split; [exact N |]); apply Eacc; exact F. }
-    eassert (Eb' : Map.Eq
-      (Map.set_union (Map.range (NewNames.generate reserved2 (BoundIn.pattern pattern))) reserved1)
-      (Map.set_union (Map.range (NewNames.generate reserved2 (BoundIn.pattern pattern))) reserved2)). {
-      split; intro F; (apply Map.union_overriding; [intros ? [] ? [] ?; reflexivity |]);
-      (apply Map.union_overriding in F as [F | F]; [left; exact F | right | intros ? [] ? [] ?; reflexivity]);
-      apply Ereserved; exact F. }
-    destruct (IHt1 _ _ Ea' _ _ Eb'); constructor; eassumption.
+        intros ->; contradiction N; apply NewNames.new_name_det]); try exact Ereserved; apply Map.eq_sym; exact Ereserved.
+    + erewrite NewNames.new_name_det. { constructor. exact Ereserved0. } exact Ereserved.
+  - destruct (IHt2 _ _ Ea _ _ Er). { constructor. } destruct Rename.pattern eqn:ER. 2: {
+      destruct Rename.pattern eqn:ER2 at 1. 2: { constructor. }
+      eapply (Rename.pattern_iff (NewNames.one_to_one_generate _ _)) in ER2.
+      eapply (@Rename.pattern_eq _ (NewNames.one_to_one_generate _ _)) in ER2; try reflexivity.
+      * eapply Rename.pattern_iff in ER2. rewrite ER2 in ER. discriminate ER.
+      * erewrite <- NewNames.generate_det. { apply Map.eq_refl. } { exact Ereserved. } apply Map.eq_refl. }
+    apply (Rename.pattern_iff (NewNames.one_to_one_generate _ _)) in ER.
+    eapply (@Rename.pattern_eq _ (NewNames.one_to_one_generate _ _)) in ER; try reflexivity; [
+      eapply Rename.pattern_iff in ER; rewrite ER; clear ER |
+      erewrite NewNames.generate_det; try apply Map.eq_refl; exact Ereserved].
+    eassert (Ea' : _); [| eassert (Er' : _); [| destruct (IHt1
+      (Map.overriding_union (Map.fold (fun k _ acc => Map.overriding_add k (NewNames.new_name
+        (Map.overriding_union reserved1 $ Map.fold (fun _ v acc0 => Map.overriding_add v tt acc0) Map.empty acc) k) acc)
+        Map.empty (BoundIn.pattern pattern)) a1)
+      (Map.overriding_union (Map.fold (fun k _ acc => Map.overriding_add k (NewNames.new_name
+        (Map.overriding_union reserved2 $ Map.fold (fun _ v acc0 => Map.overriding_add v tt acc0) Map.empty acc) k) acc)
+        Map.empty (BoundIn.pattern pattern)) a2) Ea'
+      (Map.overriding_union (Map.fold (fun _ v acc => Map.overriding_add v tt acc) Map.empty
+        (Map.fold (fun k _ acc => Map.overriding_add k (NewNames.new_name (Map.overriding_union reserved1
+          (Map.fold (fun _ v acc0 => Map.overriding_add v tt acc0) Map.empty acc)) k) acc)
+          Map.empty (BoundIn.pattern pattern))) reserved1)
+      (Map.overriding_union (Map.fold (fun _ v acc => Map.overriding_add v tt acc) Map.empty
+        (Map.fold (fun k _ acc => Map.overriding_add k (NewNames.new_name (Map.overriding_union reserved2
+          (Map.fold (fun _ v acc0 => Map.overriding_add v tt acc0) Map.empty acc)) k) acc)
+          Map.empty (BoundIn.pattern pattern))) reserved2) Er')]]. 3: { constructor. }
+    + assert (G := @NewNames.generate_det). cbn in G. erewrite G.
+      * split; intro F; apply Map.bulk_overwrite_bulk_overwrite;
+        (apply Map.bulk_overwrite_bulk_overwrite in F as [F | [N F]]; [left; exact F | right]);
+        (split; [intro I; apply N; exact I |]; apply Ea; exact F).
+      * exact Ereserved.
+      * apply Map.eq_refl.
+    + assert (G := @NewNames.generate_det). cbn in G. erewrite G.
+      * split; intro F; apply Map.bulk_overwrite_bulk_overwrite;
+        (apply Map.bulk_overwrite_bulk_overwrite in F as [F | [N F]]; [left; exact F | right]);
+        (split; [intro I; apply N; exact I |]; apply Ereserved; exact F).
+      * exact Ereserved.
+      * apply Map.eq_refl.
+    + constructor. exact Ereserved0. }
+  Unshelve.
+  - apply NewNames.one_to_one_generate.
+  - apply NewNames.one_to_one_generate.
 Qed.
 
 Lemma det
@@ -212,122 +147,257 @@ Proof.
   - unfold unshadow. destruct (det_acc A Er Et); reflexivity.
 Qed.
 
-Lemma range {acc reserved term acc' reserved' renamed}
-  (E : unshadow_acc acc reserved term = Some (acc', reserved', renamed))
-  (prev : forall x y (Fa : Map.Find acc x y), Map.In reserved y) x y (Fa : Map.Find acc' x y)
-  : Map.In reserved' y.
+Lemma bindings {acc reserved term bindings renamed}
+  (E : unshadow_acc acc reserved term = Some (bindings, renamed))
+  (prev : forall x y (Fa : Map.Find acc x y), Map.In reserved y)
+  : Map.Reflect (fun x => BoundIn.Term renamed x \/ Map.In reserved x) bindings.
 Proof.
-  generalize dependent y. generalize dependent x. generalize dependent renamed. generalize dependent reserved'.
-  generalize dependent acc'. generalize dependent reserved. generalize dependent acc. induction term; intros; cbn in *.
-  - invert E. eapply prev. exact Fa.
-  - destruct (Map.find_spec acc name) as [name' F | N]; invert E. { eapply prev. exact Fa. }
-    apply Map.in_overriding_add. apply Map.find_overriding_add in Fa as [[-> ->] | [Na Fa]]. { left. reflexivity. }
-    right. eapply prev. exact Fa.
-  - destruct (Map.find_spec acc name) as [name' F | N]; invert E. { eapply prev. exact Fa. }
-    apply Map.in_overriding_add. apply Map.find_overriding_add in Fa as [[-> ->] | [Na Fa]]. { left. reflexivity. }
-    right. eapply prev. exact Fa.
-  - destruct (unshadow_acc acc reserved term1) as [[[a1 r1] f1] |] eqn:E1. 2: { discriminate E. }
-    destruct (unshadow_acc a1 r1 term2) as [[[a2 r2] f2] |] eqn:E2; invert E. eapply IHterm2. 2: { exact E2. } 2: { exact Fa. }
-    eapply IHterm1. 2: { exact E1. } exact prev.
-  - destruct (unshadow_acc acc reserved term1) as [[[a1 r1] f1] |] eqn:E1. 2: { discriminate E. }
-    destruct (unshadow_acc (Map.overriding_add variable (NewNames.new_name r1 variable) a1)
-      (Map.overriding_add (NewNames.new_name r1 variable) tt r1) term2) as [[[a2 r2] f2] |] eqn:E2; invert E.
-    eapply IHterm2. 2: { exact E2. } 2: { exact Fa. } intros k v F. apply Map.in_overriding_add.
-    apply Map.find_overriding_add in F as [[-> ->] | [N F]]; [left | right]. { reflexivity. }
-    eapply IHterm1. 2: { exact E1. } 2: { exact F. } exact prev.
-  - destruct (unshadow_acc acc reserved term2) as [[[a2 r2] f2] |] eqn:E2. 2: { discriminate E. }
-    eassert (rew : NewNames.generate r2 (BoundIn.pattern pattern) = _). { reflexivity. }
-    simpl NewNames.generate in rew at 1. rewrite rew in E. clear rew.
-    destruct Rename.pattern as [pattern' |] eqn:R. 2: { discriminate E. }
-    destruct (unshadow_acc (Map.overriding_union (NewNames.generate r2 $ BoundIn.pattern pattern) a2)
-      (Map.overriding_union (Map.fold (fun _ v acc => Map.overriding_add v tt acc)
-        Map.empty (NewNames.generate r2 $ BoundIn.pattern pattern)) r2) term1) as [[[a1 r1] f1] |] eqn:E1; invert E.
-    eapply IHterm1. 2: { exact E1. } 2: { exact Fa. } intros k v F. apply Map.in_overriding_union.
-    apply Map.bulk_overwrite_bulk_overwrite in F as [F | [N F]]. { left. apply Map.in_range. eexists. exact F. }
-    right. eapply IHterm2. 2: { exact E2. } 2: { exact F. } exact prev.
+  generalize dependent renamed. generalize dependent bindings.
+  generalize dependent reserved. generalize dependent acc. induction term; intros; simpl unshadow_acc in *.
+  - invert E. split. { intro I. right. exact I. }
+    intros [B | I]. { invert B. } exact I.
+  - destruct (Map.find_spec acc name) as [name' F | N]; invert E.
+    split. { intro I. right. exact I. }
+    intros [B | I]. { invert B. } exact I.
+  - destruct (Map.find_spec acc name) as [name' F | N]; invert E.
+    split. { intro I. right. exact I. }
+    intros [B | I]. { invert B. } exact I.
+  - destruct unshadow_acc as [[r1 t1] |] eqn:E1 in E. 2: { discriminate E. }
+    destruct unshadow_acc as [[r2 t2] |] eqn:E2 in E; invert E. eapply IHterm1 in E1; try eassumption.
+    eapply IHterm2 in E2; try eassumption. 2: { intros. apply E1. right. eapply prev. exact Fa. } split.
+    + intro I. apply E2 in I as [B | I].
+      * left. apply BoundIn.TApA. exact B.
+      * apply E1 in I as [B | I]; [left | right].
+        { apply BoundIn.TApF. exact B. } exact I.
+    + intro UI. apply E2. destruct UI as [B | I].
+      * invert B. 2: { left. exact bound_in_argument. }
+        right. apply E1. left. exact bound_in_function.
+      * right. apply E1. right. exact I.
+  - destruct unshadow_acc as [[r1 t1] |] eqn:E1 in E. 2: { discriminate E. }
+    destruct unshadow_acc as [[r2 t2] |] eqn:E2 in E; invert E.
+    apply IHterm1 in E1. 2: { exact prev. } apply IHterm2 in E2. 2: { intros. apply Map.in_overriding_add.
+      apply Map.find_overriding_add in Fa as [[-> ->] | [Na Fa]]; [left | right]. { reflexivity. }
+      apply E1. right. eapply prev. exact Fa. } split.
+    + intro I. apply E2 in I as [B | I]. { left. apply BoundIn.TFoB. exact B. }
+      apply Map.in_overriding_add in I as [-> | I]. { left. apply BoundIn.TFoV. }
+      apply E1 in I as [B | I]. { left. apply BoundIn.TFoT. exact B. } right. exact I.
+    + intro BI. apply E2. rewrite Map.in_overriding_add.
+      destruct BI as [B | I]. 2: { right. right. apply E1. right. exact I. }
+      invert B. { right. left. reflexivity. } 2: { left. exact bound_in_body. }
+      right. right. apply E1. left. exact bound_in_type.
+  - destruct unshadow_acc as [[r2 t2] |] eqn:E2 in E. 2: { discriminate E. }
+    destruct (@Rename.pattern_spec (Map.fold (fun k _ acc => Map.overriding_add k (NewNames.new_name
+      (Map.overriding_union r2 (Map.fold (fun _ v acc' => Map.overriding_add v tt acc') Map.empty acc))
+      k) acc) Map.empty (BoundIn.pattern pattern)) (NewNames.one_to_one_generate _ _) pattern). 2: { discriminate E. }
+    destruct unshadow_acc as [[r1 t1] |] eqn:E1 in E; invert E.
+    apply IHterm2 in E2. 2: { exact prev. } apply IHterm1 in E1. 2: {
+      intros k v Fa. apply Map.in_overriding_union. rewrite Map.in_range.
+      apply Map.bulk_overwrite_bulk_overwrite in Fa as [Fa | [Na Fa]]. { left. eexists. exact Fa. }
+      right. apply E2. right. eapply prev. exact Fa. } split.
+    + intro I. apply E1 in I as [B | I]. { left. apply BoundIn.TCaB. exact B. }
+      apply Map.in_overriding_union in I as [I | I].
+      * apply Map.in_range in I as [y0 F]. eassert (I : Map.In _ _). { eexists. exact F. }
+        apply NewNames.in_generate in I. apply BoundIn.pattern_iff in I as B.
+        eapply Rename.bound_in_pattern in Y. left. apply BoundIn.TCaP. apply Y. eexists. split. { exact B. } exact F.
+      * apply E2 in I as [B | I]. { left. apply BoundIn.TCaO. exact B. } right. exact I.
+    + intro BI. apply E1. rewrite Map.in_overriding_union. rewrite Map.in_range.
+      destruct BI as [B | I]. 2: { right. right. apply E2. right. exact I. }
+      invert B. 2: { left. exact bound_in_body. } 2: { right. right. apply E2. left. exact bound_in_another_case. }
+      eapply Rename.bound_in_pattern in Y. apply Y in bound_in_pattern as [z [B F]]. right. left. eexists. exact F.
 Qed.
 
-Lemma used {acc reserved term acc' used renamed}
-  (E : unshadow_acc acc reserved term = Some (acc', used, renamed))
-  (prev : forall x y (Fa : Map.Find acc x y), Map.In reserved y)
-  : Map.Reflect (fun x => UsedIn.Term renamed x \/ BoundIn.Term renamed x \/ Map.In reserved x) used.
+
+
+Lemma wf_spec acc reserved t
+  : Reflect.Option
+    (fun _ => WellFormed.AllPatternsIn t /\ forall x (U : UsedIn.Term t x), Map.In acc x)
+    (unshadow_acc acc reserved t).
 Proof.
-  assert (R := range E prev). generalize dependent renamed. generalize dependent used.
-  generalize dependent acc'. generalize dependent reserved. generalize dependent acc. induction term; intros.
-  - cbn in E. invert E. split. { intro I. right. right. exact I. }
-    intros [U | [B | I]]. { invert U. } { invert B. } exact I.
-  - cbn in E. destruct (Map.find_spec acc name) as [name' F | N]; invert E.
-    + split. { intro I. right. right. exact I. }
-      intros [U | [B | I]]. { invert U. eapply R. exact F. } { invert B. } exact I.
-    + intro x. rewrite Map.in_overriding_add. split. { intros [-> | I]. { left. constructor. } right. right. exact I. }
-      intros [U | [B | I]]; [left | | right]. { invert U. reflexivity. } { invert B. } exact I.
-  - cbn in E. destruct (Map.find_spec acc name) as [name' F | N]; invert E.
-    + split. { intro I. right. right. exact I. }
-      intros [U | [B | I]]. { invert U. eapply R. exact F. } { invert B. } exact I.
-    + intro x. rewrite Map.in_overriding_add. split. { intros [-> | I]. { left. constructor. } right. right. exact I. }
-      intros [U | [B | I]]; [left | | right]. { invert U. reflexivity. } { invert B. } exact I.
-  - cbn in E. destruct unshadow_acc as [[[a1 r1] t1] |] eqn:E1 in E. 2: { discriminate E. }
-    destruct unshadow_acc as [[[a2 r2] t2] |] eqn:E2 in E; invert E. assert (R1 := range E1 prev).
-    eapply IHterm1 in E1; try eassumption. eapply IHterm2 in E2; try eassumption. split.
-    + intro I. apply E2 in I as [U | [B | I]].
-      * left. apply UsedIn.ApA. exact U.
-      * right. left. apply BoundIn.TApA. exact B.
-      * apply E1 in I as [U | [B | I]]; [left | right; left | right; right].
-        { apply UsedIn.ApF. exact U. } { apply BoundIn.TApF. exact B. } exact I.
-    + intro UI. apply E2. destruct UI as [U | [B | I]].
-      * invert U. 2: { left. exact used_in_argument. } right. right. apply E1. left. exact used_in_function.
-      * invert B. 2: { right. left. exact bound_in_argument. }
-        right. right. apply E1. right. left. exact bound_in_function.
-      * right. right. apply E1. right. right. exact I.
-  - rewrite unshadow_acc_for in E. destruct unshadow_acc as [[[a1 r1] t1] |] eqn:E1 in E. 2: { discriminate E. }
-    destruct unshadow_acc as [[[a2 r2] t2] |] eqn:E2 in E; invert E. assert (R1 := range E1 prev).
-    eapply IHterm1 in E1; try eassumption. eapply IHterm2 in E2; try eassumption. 2: { intros. apply Map.in_overriding_add.
-      apply Map.find_overriding_add in Fa as [[-> ->] | [Na Fa]]; [left | right]. { reflexivity. } eapply R1. exact Fa. }
-    split.
-    + intro I. destruct (String.eqb_spec x (NewNames.new_name r1 variable)). { subst. right. left. apply BoundIn.TFoV. }
-      apply E2 in I as [U | [B | I]]. { left. apply UsedIn.FoB; assumption. } { right. left. apply BoundIn.TFoB. exact B. }
-      apply Map.in_overriding_add in I as [C | I]. { apply n in C as []. }
-      apply E1 in I as [U | [B | I]]. { left. apply UsedIn.FoT. exact U. } { right. left. apply BoundIn.TFoT. exact B. }
-      right. right. exact I.
-    + intro UBI. apply E2. unfold Map.set_add. rewrite Map.in_overriding_add. destruct UBI as [U | [B | I]].
-      * invert U. 2: { left. exact used_in_body. } right. right. right. apply E1. left. exact used_in_type.
-      * invert B. { right. right. left. reflexivity. } 2: { right. left. exact bound_in_body. }
-        right. right. right. apply E1. right. left. exact bound_in_type.
-      * right. right. right. apply E1. right. right. exact I.
-  - rewrite unshadow_acc_cas in E. destruct unshadow_acc as [[[a1 r1] t1] |] eqn:E1 in E. 2: { discriminate E. }
-    eassert (O2O : _); [| destruct (@Rename.pattern_spec (NewNames.generate r1 (BoundIn.pattern pattern))
-      O2O pattern) as [renamed_pattern RP | NR]; [| discriminate E]]. { apply NewNames.one_to_one_generate. }
-    destruct unshadow_acc as [[[a2 r2] t2] |] eqn:E2 in E; invert E. assert (R1 := range E1 prev).
-    eapply IHterm2 in E1; try eassumption. eapply IHterm1 in E2; try eassumption. 2: { intros. apply Map.in_overriding_union.
-      apply Map.bulk_overwrite_bulk_overwrite in Fa as [Fa | [Na Fa]]. 2: { right. eapply R1. exact Fa. }
-      left. apply Map.in_range. eexists. exact Fa. }
-    split.
-    + (* If `x` is in the second output of the `unshadow` function (`used`), then
-       * it's either used in the renamed term, bound in it, or an extra in the original `reserved`: *)
-      intro I. destruct (BoundIn.pattern_spec renamed_pattern x). { right. left. apply BoundIn.TCaP. exact Y. }
-      (* Use the inductive hypothesis from recursing down the body of the case expression: *)
-      apply E2 in I as [U | [B | I]]. { left. apply UsedIn.CaB; assumption. } { right. left. apply BoundIn.TCaB. exact B. }
-      (* Most of those were easy, but the one in which `x` was an extra in `reserved` is more tricky, since
-       * either `x` was bound in `pattern` (i.e. the case pattern to match against) and renamed,
-       * or `x` was an extra in the _body_'s (temporary) reserved set: *)
-      apply Map.in_overriding_union in I as [I | I]. {
-        (* `x` was bound in `pattern` (i.e. the case pattern to match against) and renamed,
-         * but we know that `x` wasn't bound in the renamed `pattern`: *)
-        apply Map.in_range in I as [z F]. contradiction N. eapply Rename.bound_in_pattern. { eassumption. }
-        eexists. split. 2: { exact F. } apply BoundIn.pattern_iff. eapply NewNames.in_generate. eexists. exact F. }
-      apply E1 in I as [U | [B | I]].
-      * left. apply UsedIn.CaO. exact U.
-      * right. left. apply BoundIn.TCaO. exact B.
-      * right. right. exact I.
-    + intro UBI. apply E2. unfold Map.set_union. rewrite Map.in_overriding_union.
-      rewrite Map.in_range. destruct UBI as [U | [B | I]].
-      * invert U. { left. exact used_in_body. } right. right. right. apply E1. left. exact used_in_another_case.
-      * invert B.
-        -- right. right. left. eapply Rename.bound_in_pattern in bound_in_pattern as [z [B F]]. 2: { eassumption. }
-           eexists. exact F.
-        -- right. left. exact bound_in_body.
-        -- right. right. right. apply E1. right. left. exact bound_in_other_cases.
-      * right. right. right. apply E1. right. right. exact I.
+  generalize dependent reserved. generalize dependent acc. induction t; intros; cbn in *.
+  - constructor. split; intros. { constructor. } invert U.
+  - destruct (Map.find_spec acc name); constructor.
+    + split; intros. { constructor. } invert U. eexists. exact Y.
+    + intros _ [_ C]. edestruct C. { constructor. } apply N in H as [].
+  - destruct (Map.find_spec acc name); constructor.
+    + split; intros. { constructor. } invert U. eexists. exact Y.
+    + intros _ [_ C]. edestruct C. { constructor. } apply N in H as [].
+  - destruct (IHt1 acc reserved) as [[r1 t1'] [WF1 IH1] |]. 2: {
+      constructor. intros pair [WF C]. invert WF. apply N. { exact pair. }
+      split. { exact APf. } intros. apply C. apply UsedIn.ApF. exact U. }
+    destruct (IHt2 acc r1) as [[r2 t2'] [WF2 IH2] |]; constructor.
+    + constructor. { constructor; assumption. } intros. invert U; [apply IH1 | apply IH2]; assumption.
+    + intros pair [WF C]. invert WF. apply N. { exact pair. }
+      split. { exact APa. } intros. apply C. apply UsedIn.ApA. exact U.
+  - destruct (IHt1 acc reserved) as [[r1 t1'] [WF1 IH1] |]. 2: {
+      constructor. intros pair [WF C]. invert WF. apply N. { exact pair. }
+      split. { exact APt. } intros. apply C. apply UsedIn.FoT. exact U. }
+    destruct (IHt2 (Map.overriding_add variable (NewNames.new_name r1 variable) acc)
+      (Map.overriding_add (NewNames.new_name r1 variable) tt r1)) as [[r2 t2'] [WF2 IH2] |]; constructor.
+    + split. { constructor; assumption. } intros. invert U. { apply IH1. exact used_in_type. }
+      apply IH2 in used_in_body. apply Map.in_overriding_add in used_in_body as [-> | I]. 2: { exact I. }
+      contradiction not_shadowed. reflexivity.
+    + intros pair [WF C]. invert WF. apply N. { exact pair. }
+      split. { exact APb. } intros. apply Map.in_overriding_add.
+      destruct (String.eqb_spec x variable); [left | right]. { assumption. } apply C. apply UsedIn.FoB; assumption.
+  - destruct (IHt2 acc reserved) as [[r2 t2'] [WF2 IH2] |]. 2: {
+      constructor. intros pair [WF C]. invert WF. apply N. { exact pair. }
+      split. { exact APo. } intros. apply C. apply UsedIn.CaO. exact U. }
+    destruct (@Rename.pattern_spec (Map.fold (fun k _ acc' => Map.overriding_add k (NewNames.new_name
+      (Map.overriding_union r2 (Map.fold (fun _ v acc'' => Map.overriding_add v tt acc'') Map.empty acc'))
+      k) acc') Map.empty (BoundIn.pattern pattern)) (NewNames.one_to_one_generate _ _) pattern). 2: {
+      constructor. intros pair [WF C]. invert WF. eassert (RC : Rename.CompatiblePattern _ _). 2: {
+        apply Rename.pattern_iff_compatible in RC as [O2O [renamed R]].
+        eapply Rename.pattern_eq in R; try reflexivity. { apply N in R as []. } apply Map.eq_refl. }
+      invert WFp; constructor. { apply NewNames.one_to_one_generate. } {
+        apply NewNames.in_generate. apply Map.in_singleton. reflexivity. }
+      invert move_or_reference_well_formed; constructor; (split; [apply NewNames.one_to_one_generate |]);
+      (split; [exact strict_well_formed |]); intros k [] F; apply Map.find_domain;
+      apply NewNames.in_generate; cbn; exists tt; exact F. }
+    eassert (RC : Rename.CompatiblePattern _ _). { apply Rename.pattern_iff_compatible. do 2 eexists. exact Y. }
+    destruct (IHt1
+      (Map.overriding_union (Map.fold (fun k _ acc' => Map.overriding_add k (NewNames.new_name (Map.overriding_union r2
+        (Map.fold (fun _ v acc'' => Map.overriding_add v tt acc'') Map.empty acc')) k) acc') Map.empty (BoundIn.pattern pattern)) acc)
+      (Map.overriding_union (Map.fold (fun _ v acc' => Map.overriding_add v tt acc') Map.empty (Map.fold
+        (fun k _ acc' => Map.overriding_add k (NewNames.new_name (Map.overriding_union r2 (Map.fold
+          (fun _ v acc'' => Map.overriding_add v tt acc'') Map.empty acc')) k) acc')
+        Map.empty (BoundIn.pattern pattern))) r2)) as [[r1 t1'] [WF1 IH1] |]; constructor.
+    + constructor. { constructor; try assumption. invert RC; constructor. invert C; constructor; apply CS. }
+      intros z U. invert U. 2: { apply IH2. exact used_in_another_case. } apply IH1 in used_in_body.
+      apply Map.in_overriding_union in used_in_body as [I | I]. 2: { exact I. }
+      apply NewNames.in_generate in I. apply BoundIn.pattern_iff in I. apply not_shadowed in I as [].
+    + intros pair [WF C]. invert WF. apply N. { exact pair. } split. { exact APb. } intros.
+      apply Map.in_overriding_union. destruct (BoundIn.pattern_spec pattern x0); [left | right].
+      * apply NewNames.in_generate. apply BoundIn.pattern_iff. exact Y0.
+      * apply C. apply UsedIn.CaB; assumption.
+Qed.
+
+Lemma disjoint_used {acc reserved term reserved' renamed}
+  (E : unshadow_acc acc reserved term = Some (reserved', renamed))
+  (prev : forall x y (Fa : Map.Find acc x y), Map.In reserved y)
+  {y} (I : Map.In reserved y) (U : UsedIn.Term renamed y)
+  : exists x, Map.Find acc x y.
+Proof.
+  generalize dependent y. generalize dependent renamed. generalize dependent reserved'.
+  generalize dependent reserved. generalize dependent acc. induction term; intros; cbn in *.
+  - invert E. invert U.
+  - destruct (Map.find_spec acc name); invert E. invert U. eexists. exact Y.
+  - destruct (Map.find_spec acc name); invert E. invert U. eexists. exact Y.
+  - destruct unshadow_acc as [[r1 t1] |] eqn:E1 in E. 2: { discriminate E. }
+    destruct unshadow_acc as [[r2 t2] |] eqn:E2 in E; invert E.
+    invert U. { eapply IHterm1. { exact prev. } { exact E1. } { exact I. } exact used_in_function. }
+    eapply IHterm2. 2: { exact E2. } 3: { exact used_in_argument. }
+    + intros. eapply bindings. { exact E1. } { exact prev. } right. eapply prev. exact Fa.
+    + eapply bindings. { exact E1. } { exact prev. } right. exact I.
+  - destruct unshadow_acc as [[r1 t1] |] eqn:E1 in E. 2: { discriminate E. }
+    destruct unshadow_acc as [[r2 t2] |] eqn:E2 in E; invert E.
+    invert U. { eapply IHterm1. { exact prev. } { exact E1. } { exact I. } exact used_in_type. }
+    eapply IHterm2 in E2 as [x IH2]. 4: { exact used_in_body. }
+    + apply Map.find_overriding_add in IH2 as [[-> ->] | [N F]]. { contradiction not_shadowed. reflexivity. } eexists. exact F.
+    + intros. apply Map.in_overriding_add. apply Map.find_overriding_add in Fa as [[-> ->] | [Na Fa]]; [left | right]. { reflexivity. }
+      eapply bindings. { exact E1. } { exact prev. } right. eapply prev. exact Fa.
+    + apply Map.in_overriding_add. right. eapply bindings. { exact E1. } { exact prev. } right. exact I.
+  - destruct unshadow_acc as [[r2 t2] |] eqn:E2 in E. 2: { discriminate E. }
+    destruct (@Rename.pattern_spec (Map.fold (fun k _ acc' => Map.overriding_add k (NewNames.new_name
+      (Map.overriding_union r2 (Map.fold (fun _ v acc'' => Map.overriding_add v tt acc'') Map.empty acc'))
+      k) acc') Map.empty (BoundIn.pattern pattern)) (NewNames.one_to_one_generate _ _) pattern). 2: { discriminate E. }
+    destruct unshadow_acc as [[r1 t1] |] eqn:E1 in E; invert E.
+    invert U. 2: { eapply IHterm2. { exact prev. } { exact E2. } { exact I. } exact used_in_another_case. }
+    eapply IHterm1 in E1 as [z IH1]. 4: { exact used_in_body. }
+    + apply Map.bulk_overwrite_bulk_overwrite in IH1 as [F | [N F]]. 2: { eexists. exact F. }
+      eassert (I' : Map.In _ _). { eexists. exact F. } apply NewNames.in_generate in I'. apply BoundIn.pattern_iff in I' as B.
+      contradiction not_shadowed. eapply Rename.bound_in_pattern. { exact Y. } eexists. split. { exact B. } exact F.
+    + intros k v F. apply Map.in_overriding_union.
+      apply Map.bulk_overwrite_bulk_overwrite in F as [F | [N F]]. { left. apply Map.in_range. eexists. exact F. }
+      right. eapply bindings. { exact E2. } { exact prev. } right. eapply prev. exact F.
+    + apply Map.in_overriding_union. right. eapply bindings. { exact E2. } { exact prev. } right. exact I.
+Qed.
+
+Lemma disjoint_bound {acc reserved term reserved' renamed}
+  (E : unshadow_acc acc reserved term = Some (reserved', renamed))
+  (prev : forall x y (Fa : Map.Find acc x y), Map.In reserved y)
+  {x} (I : Map.In reserved x) (B : BoundIn.Term renamed x)
+  : False.
+Proof.
+  generalize dependent x. generalize dependent renamed. generalize dependent reserved'.
+  generalize dependent reserved. generalize dependent acc. induction term; intros; cbn in *.
+  - invert E. invert B.
+  - destruct (Map.find_spec acc name); invert E. invert B.
+  - destruct (Map.find_spec acc name); invert E. invert B.
+  - destruct unshadow_acc as [[r1 t1] |] eqn:E1 in E. 2: { discriminate E. }
+    destruct unshadow_acc as [[r2 t2] |] eqn:E2 in E; invert E.
+    invert B. { eapply IHterm1. { exact prev. } { exact E1. } { exact I. } exact bound_in_function. }
+    eapply IHterm2. 2: { exact E2. } 3: { exact bound_in_argument. }
+    + intros. eapply bindings. { exact E1. } { exact prev. } right. eapply prev. exact Fa.
+    + eapply bindings. { exact E1. } { exact prev. } right. exact I.
+  - destruct unshadow_acc as [[r1 t1] |] eqn:E1 in E. 2: { discriminate E. }
+    destruct unshadow_acc as [[r2 t2] |] eqn:E2 in E; invert E. invert B.
+    + eapply NewNames.not_in_new_name. eapply bindings. { exact E1. } { exact prev. } right. exact I.
+    + eapply IHterm1. { exact prev. } { exact E1. } { exact I. } exact bound_in_type.
+    + eapply IHterm2 in E2 as []. 3: { exact bound_in_body. }
+      * intros. apply Map.in_overriding_add. apply Map.find_overriding_add in Fa as [[-> ->] | [Na Fa]]. { left. reflexivity. }
+        right. eapply bindings. { exact E1. } { exact prev. } right. eapply prev. exact Fa.
+      * apply Map.in_overriding_add. right. eapply bindings. { exact E1. } { exact prev. } right. exact I.
+  - destruct unshadow_acc as [[r2 t2] |] eqn:E2 in E. 2: { discriminate E. }
+    destruct (@Rename.pattern_spec (Map.fold (fun k _ acc' => Map.overriding_add k (NewNames.new_name
+      (Map.overriding_union r2 (Map.fold (fun _ v acc'' => Map.overriding_add v tt acc'') Map.empty acc'))
+      k) acc') Map.empty (BoundIn.pattern pattern)) (NewNames.one_to_one_generate _ _) pattern). 2: { discriminate E. }
+    destruct unshadow_acc as [[r1 t1] |] eqn:E1 in E; invert E. invert B.
+    + apply (Rename.bound_in_pattern Y) in bound_in_pattern as [z [B F]]. eapply NewNames.not_in_generate. 2: { eexists. exact F. }
+      eapply bindings. { exact E2. } { exact prev. } right. exact I.
+    + eapply IHterm1 in E1 as []. 3: { exact bound_in_body. }
+      * intros k v F. apply Map.in_overriding_union. rewrite Map.in_range.
+        apply Map.bulk_overwrite_bulk_overwrite in F as [F | [N F]]. { left. eexists. exact F. }
+        right. eapply bindings. { exact E2. } { exact prev. } right. eapply prev. exact F.
+      * apply Map.in_overriding_union. rewrite Map.in_range. right. eapply bindings. { exact E2. } { exact prev. } right. exact I.
+    + eapply IHterm2. { exact prev. } { exact E2. } { exact I. } exact bound_in_another_case.
+Qed.
+
+Lemma used_reserved {acc reserved term reserved' renamed}
+  (E : unshadow_acc acc reserved term = Some (reserved', renamed))
+  (prev : forall x y (Fa : Map.Find acc x y), Map.In reserved y)
+  {x} (U : UsedIn.Term renamed x)
+  : Map.In reserved' x.
+Proof.
+  generalize dependent x. generalize dependent renamed. generalize dependent reserved'.
+  generalize dependent reserved. generalize dependent acc. induction term; intros; cbn in *.
+  - invert E. invert U.
+  - destruct (Map.find_spec acc name); invert E. invert U. eapply prev. exact Y.
+  - destruct (Map.find_spec acc name); invert E. invert U. eapply prev. exact Y.
+  - destruct unshadow_acc as [[r1 t1] |] eqn:E1 in E. 2: { discriminate E. }
+    destruct unshadow_acc as [[r2 t2] |] eqn:E2 in E; invert E.
+    eassert (prev' : forall k v (F : Map.Find acc k v), Map.In r1 v). {
+      intros k v F. eapply bindings; try eassumption. right. eapply prev. exact F. }
+    invert U. 2: { eapply IHterm2. 2: { eassumption. } 2: { eassumption. } exact prev'. }
+    eapply IHterm1 in E1; try eassumption. eapply bindings; try eassumption. right. exact E1.
+  - destruct unshadow_acc as [[r1 t1] |] eqn:E1 in E. 2: { discriminate E. }
+    eassert (prev' : forall k v (F : Map.Find (Map.overriding_add variable (NewNames.new_name r1 variable) acc) k v),
+      Map.In (Map.overriding_add (NewNames.new_name r1 variable) tt r1) v). {
+      intros k v F. apply Map.in_overriding_add. apply Map.find_overriding_add in F as [[-> ->] | [N F]]. { left. reflexivity. }
+      right. eapply bindings. { exact E1. } { exact prev. } right. eapply prev. exact F. }
+    destruct unshadow_acc as [[r2 t2] |] eqn:E2 in E; invert E. invert U. 2: {
+      eapply IHterm2. 2: { exact E2. } 2: { exact used_in_body. } exact prev'. }
+    eapply IHterm1 in E1; try eassumption. eapply bindings; try eassumption.
+    right. apply Map.in_overriding_add. right. exact E1.
+  - destruct unshadow_acc as [[r2 t2] |] eqn:E2 in E. 2: { discriminate E. }
+    destruct (@Rename.pattern_spec (Map.fold (fun k _ acc' => Map.overriding_add k (NewNames.new_name
+      (Map.overriding_union r2 (Map.fold (fun _ v acc'' => Map.overriding_add v tt acc'') Map.empty acc'))
+      k) acc') Map.empty (BoundIn.pattern pattern)) (NewNames.one_to_one_generate _ _) pattern). 2: { discriminate E. }
+    eassert (prev' : forall z y,
+      Map.Find (Map.overriding_union (Map.fold (fun k _ acc' => Map.overriding_add k (NewNames.new_name
+        (Map.overriding_union r2 (Map.fold (fun _ v acc1 => Map.overriding_add v tt acc1) Map.empty acc'))
+        k) acc') Map.empty (BoundIn.pattern pattern)) acc) z y ->
+      exists v : unit,
+      Map.Find (Map.overriding_union (Map.fold (fun (_ v0 : String.string) (acc' : Map.to unit) =>
+        Map.overriding_add v0 tt acc') Map.empty (Map.fold (fun k _ acc' => Map.overriding_add k (NewNames.new_name
+        (Map.overriding_union r2 (Map.fold (fun _ v0 acc1 => Map.overriding_add v0 tt acc1) Map.empty acc'))
+        k) acc') Map.empty (BoundIn.pattern pattern))) r2) y v). {
+      intros k v F. apply Map.in_overriding_union. rewrite Map.in_range.
+      apply Map.bulk_overwrite_bulk_overwrite in F as [F | [N F]]. { left. eexists. exact F. }
+      right. eapply bindings. { exact E2. } { exact prev. } right. eapply prev. exact F. }
+    destruct unshadow_acc as [[r1 t1] |] eqn:E1 in E; invert E. invert U. {
+      eapply IHterm1. 2: { exact E1. } 2: { exact used_in_body. } exact prev'. }
+    eapply IHterm2 in E2; try eassumption. eapply bindings; try eassumption.
+    right. apply Map.in_overriding_union. right. exact E2.
 Qed.
 
 
@@ -345,24 +415,90 @@ Inductive Unshadowed : Term.term -> Prop :=
       (disj_f_a : forall x (Bf : BoundIn.Term function x) (Ua : UsedIn.Term argument x), False)
       (disj_a_f : forall x (Ba : BoundIn.Term argument x) (Uf : UsedIn.Term function x), False)
       : Unshadowed (Term.App function argument)
+  | For
+      {type} (Ut : Unshadowed type)
+      {body} (Ub : Unshadowed body)
+      (disj_t_b : forall x (Bt : BoundIn.Term type x) (Ub : UsedIn.Term body x), False)
+      (disj_b_t : forall x (Bb : BoundIn.Term body x) (Ut : UsedIn.Term type x), False) {variable}
+      (Nt : forall (B : BoundIn.Term type variable), False)
+      (Nb : forall (B : BoundIn.Term body variable), False)
+      : Unshadowed (Term.For variable type body)
+  | Cas
+      {body_if_match} (Ub : Unshadowed body_if_match)
+      {other_cases} (Uo : Unshadowed other_cases)
+      (disj_b_o : forall x (Bb : BoundIn.Term body_if_match x) (Uo : UsedIn.Term other_cases x), False)
+      (disj_o_b : forall x (Bo : BoundIn.Term other_cases x) (Ub : UsedIn.Term body_if_match x), False) {pattern}
+      (Nb : forall x (Bp : BoundIn.Pattern pattern x) (Bt : BoundIn.Term body_if_match x), False)
+      (No : forall x (Bp : BoundIn.Pattern pattern x) (Bo : BoundIn.Term other_cases x), False)
+      : Unshadowed (Term.Cas pattern body_if_match other_cases)
   .
 
-Lemma unshadowed_acc {acc reserved t acc' reserved' renamed}
-  (E : unshadow_acc acc reserved t = Some (acc', reserved', renamed))
+Lemma unshadowed_acc {acc reserved t reserved' renamed}
+  (E : unshadow_acc acc reserved t = Some (reserved', renamed))
   (prev : forall x y (Fa : Map.Find acc x y), Map.In reserved y)
   : Unshadowed renamed.
 Proof.
-  (*assert (R := range E prev). assert (U := used E prev).*)
-  generalize dependent renamed. generalize dependent reserved'. generalize dependent acc'.
-  generalize dependent reserved. generalize dependent acc. induction t; intros.
-  - cbn in E. invert E. constructor.
-  - cbn in E. destruct (Map.find_spec acc name); cbn in E; invert E; constructor.
-  - cbn in E. destruct (Map.find_spec acc name); cbn in E; invert E; constructor.
-  - cbn in E. destruct (unshadow_acc acc reserved t1) as [[[acc1 reserved1] renamed1] |] eqn:E1. 2: { discriminate E. }
-    destruct (unshadow_acc acc1 reserved1 t2) as [[[acc2 reserved2] renamed2] |] eqn:E2; invert E.
-    specialize (IHt1 _ _ prev _ _ _ E1). eassert (prev1 : _); [| specialize (IHt2 _ _ prev1 _ _ _ E2)]. {
-      intros. eapply range. { eassumption. } { exact prev. } exact Fa. }
-    constructor; try assumption; intros. Abort.
+  generalize dependent renamed. generalize dependent reserved'.
+  generalize dependent reserved. generalize dependent acc. induction t; intros; cbn in *.
+  - invert E. constructor.
+  - destruct (Map.find_spec acc name); cbn in E; invert E; constructor.
+  - destruct (Map.find_spec acc name); cbn in E; invert E; constructor.
+  - destruct unshadow_acc as [[reserved1 renamed1] |] eqn:E1 in E. 2: { discriminate E. }
+    destruct unshadow_acc as [[reserved2 renamed2] |] eqn:E2 in E; invert E.
+    specialize (IHt1 _ _ prev _ _ E1). eassert (prev' : _); [| specialize (IHt2 _ _ prev' _ _ E2)]. {
+      intros. eapply bindings. { exact E1. } { exact prev. } right. eapply prev. exact Fa. }
+    constructor; try assumption; intros.
+    + eapply disjoint_bound; try exact Bf; try eassumption.
+      assert (I : Map.In reserved1 x). { eapply bindings. { exact E1. } { exact prev. } left. exact Bf. }
+      destruct (disjoint_used E2 prev' I Ua) as [z F]. eapply prev. exact F.
+    + eapply disjoint_bound; try exact Ba; try eassumption.
+      eapply used_reserved. 3: { exact Uf. } { eassumption. } exact prev.
+  - destruct unshadow_acc as [[reserved1 renamed1] |] eqn:E1 in E. 2: { discriminate E. }
+    destruct unshadow_acc as [[reserved2 renamed2] |] eqn:E2 in E; invert E.
+    specialize (IHt1 _ _ prev _ _ E1). eassert (prev' : _); [| specialize (IHt2 _ _ prev' _ _ E2)]. {
+      intros. apply Map.in_overriding_add. apply Map.find_overriding_add in Fa as [[-> ->] | [Na Fa]]. { left. reflexivity. }
+      right. eapply bindings. { exact E1. } { exact prev. } right. eapply prev. exact Fa. }
+    constructor; try assumption; intros.
+    + eapply disjoint_bound; try exact Bt; try eassumption.
+      assert (I : Map.In reserved1 x). { eapply bindings. { exact E1. } { exact prev. } left. exact Bt. }
+      eassert (I' : _); [| destruct (disjoint_used E2 prev' I' Ub) as [z F]]. { apply Map.in_overriding_add. right. exact I. }
+      apply Map.find_overriding_add in F as [[-> ->] | [N F]]. { apply NewNames.not_in_new_name in I as []. } eapply prev. exact F.
+    + eapply disjoint_bound; try exact Ba; try eassumption. apply Map.in_overriding_add.
+      destruct (String.eqb_spec x (NewNames.new_name reserved1 variable)); [left | right]. { assumption. }
+      eapply used_reserved. 3: { exact Ut. } { eassumption. } exact prev.
+    + eapply NewNames.not_in_new_name. eapply bindings. 3: { left. exact B. } { eassumption. } exact prev.
+    + eapply disjoint_bound. { exact E2. } { exact prev'. } 2: { exact B. } apply Map.in_overriding_add. left. reflexivity.
+  - destruct unshadow_acc as [[reserved2 renamed2] |] eqn:E2 in E. 2: { discriminate E. }
+    destruct (@Rename.pattern_spec (Map.fold (fun k _ acc' => Map.overriding_add k (NewNames.new_name
+      (Map.overriding_union reserved2 (Map.fold (fun _ v acc'' => Map.overriding_add v tt acc'') Map.empty acc'))
+      k) acc') Map.empty (BoundIn.pattern pattern)) (NewNames.one_to_one_generate _ _) pattern). 2: { discriminate E. }
+    destruct unshadow_acc as [[reserved1 renamed1] |] eqn:E1 in E; invert E.
+    specialize (IHt2 _ _ prev _ _ E2). eassert (prev' : _); [| specialize (IHt1 _ _ prev' _ _ E1)]. {
+      intros k v F. apply Map.in_overriding_union. rewrite Map.in_range.
+      apply Map.bulk_overwrite_bulk_overwrite in F as [F | [N F]]. { left. eexists. exact F. }
+      right. eapply bindings. { exact E2. } { exact prev. } right. eapply prev. exact F. }
+    constructor; try assumption; intros.
+    + eapply disjoint_bound; try exact Bb; try eassumption. apply Map.in_overriding_union. rewrite Map.in_range.
+      right. eapply used_reserved. { eassumption. } { exact prev. } exact Uo.
+    + eapply disjoint_bound; try exact Bo; try eassumption.
+      assert (I : Map.In reserved2 x0). { eapply bindings. { exact E2. } { exact prev. } left. exact Bo. }
+      eassert (I' : _); [| destruct (disjoint_used E1 prev' I' Ub) as [z F]]. { apply Map.in_overriding_union. right. exact I. }
+      apply Map.bulk_overwrite_bulk_overwrite in F as [F | [N F]]. 2: { eapply prev. exact F. }
+      eassert (IR : Map.InRange _ _). { eexists. exact F. } eapply NewNames.not_in_generate in IR as []. exact I.
+    + apply (Rename.bound_in_pattern Y) in Bp as [z [B F]].
+      eapply disjoint_bound. { exact E1. } { exact prev'. } 2: { exact Bt. }
+      apply Map.in_overriding_union. left. apply Map.in_range. eexists. exact F.
+    + apply (Rename.bound_in_pattern Y) in Bp as [z [B F]].
+      eapply NewNames.not_in_generate. 2: { eexists. exact F. }
+      eapply bindings. 3: { left. exact Bo. } { exact E2. } exact prev.
+Qed.
+
+Lemma unshadowed {reserved t renamed} (E : unshadow reserved t = Some renamed)
+  : Unshadowed renamed.
+Proof.
+  cbn in E. destruct unshadow_acc as [[? ?] |] eqn:Ea; invert E. eapply unshadowed_acc in Ea. { exact Ea. }
+  intros k v F. apply Map.to_self_to_self in F as [I ->]. exact I.
+Qed.
 
 
 
